# E1.17 Exponential Growth and Decay

## Understanding Exponential Growth and Decay

Exponential growth and decay occur when a quantity changes by a constant percentage over equal time periods.

### Exponential Growth Formula
$A = P(1 + r)^t $
Where:
- $ \text{A = final amount}$
- $ \text{P = initial amount}$
- $ \text{r} = \text{growth rate (as decimal)}$
- $ \text{t = time periods}$

### Exponential Decay Formula
$ A = P(1 - r)^t $
Where:
- $\text{r = decay rate (as decimal)}$



## Applications

### Depreciation
**Example**: A car worth \$20,000 depreciates at 15% per year. Find its value after 4 years.
- $ \text{r = 0.15 , t = 4} $
- $ \text{A = }20000(1 - 0.15)^4 = 20000(0.85)^4 $
- $ \text{A = }20000 \times 0.522 = \text{10,440} $

### Population Growth
**Example**: A population of 5000 grows at 8% per year. Find population after 6 years.
- $ \text{r = 0.08 , t = 6} $
- $ \text{A = }5000(1 + 0.08)^6 = 5000(1.08)^6 $
- $ \text{A = }5000 \times 1.587 = 7935 $

# E1.18 Surds

## 1. Understanding and Simplifying Surds

A surd is an irrational number expressed as a root, most commonly a square root.

### Simplifying Surds
$ \sqrt{a \times b} = \sqrt{a} \times \sqrt{b} $

$\text{Example: Simplify}  \sqrt{20} $
 
- $\sqrt{20} = \sqrt{4 \times 5} = \sqrt{4} \times \sqrt{5} = 2\sqrt{5} $


$\text{Example: Simplify} \sqrt{200} - \sqrt{32} $

- $\sqrt{200} = \sqrt{100 \times 2} = 10\sqrt{2} $ 
- $ \sqrt{32} = \sqrt{16 \times 2} = 4\sqrt{2}$
- $10\sqrt{2} - 4\sqrt{2} = 6\sqrt{2} $

## 2. Rationalising the Denominator

Rationalising means eliminating surds from the denominator of a fraction.

### Simple Denominators


$\text{Example: Rationalise  }  \frac{10}{\sqrt{5}} $

- $ \frac{10}{\sqrt{5}} \times \frac{\sqrt{5}}{\sqrt{5}} $
- $ \frac{10\sqrt{5}}{5} = 2\sqrt{5} $

### Binomial Denominators
$\text{Use the conjugate: } \frac{1}{a + \sqrt{b}} \times \frac{a - \sqrt{b}}{a - \sqrt{b}} $

$Example: Rationalise \frac{1}{-1 + \sqrt{3}} $
- $\text{Multiply numerator and denominator by conjugate}  -1 - \sqrt{3} :$
- $\frac{1}{-1 + \sqrt{3}} \times \frac{-1 - \sqrt{3}}{-1 - \sqrt{3}} = \frac{-1 - \sqrt{3}}{(-1)^2 - (\sqrt{3})^2}$
- $ = \frac{-1 - \sqrt{3}}{1 - 3} = \frac{-1 - \sqrt{3}}{-2} = \frac{1 + \sqrt{3}}{2} $

## Key Points to Remember

### Exponential Growth/Decay
- Growth: (1 + r), Decay: (1 - r)
- Rate r must be expressed as decimal
- Time periods must be consistent
- Knowledge of e is not required for this level

### Surds
- Always simplify surds completely
- For binomial denominators, use the conjugate
- $\text{The conjugate of   } a + \sqrt{b}  \text{   is    } a - \sqrt{b} $
- Check your answer by verifying the denominator is rational

These skills are essential for financial calculations, population studies, and advanced algebraic manipulation.