# E2.5 Equations

## 1. Constructing Expressions, Equations, and Formulas

Translate word problems into algebraic form.

**Example**: Write an expression for the product of two consecutive even numbers.
- Let the first even number be $2n$
- The next consecutive even number is $2n + 2$
- Product: $2n(2n + 2) = 4n^2 + 4n$

**Example**: Construct simultaneous equations for: "The sum of two numbers is 15, and their difference is 3."
- Let the numbers be $x$ and $y$
- Equations: $x + y = 15$, $x - y = 3$

## 2. Solving Linear Equations in One Unknown

Isolate the variable using inverse operations.

**Example**: Solve $3x + 4 = 10$
- $3x = 10 - 4$
- $3x = 6$
- $x = 2$

**Example**: Solve $5 - 2x = 3(x + 7)$
- $5 - 2x = 3x + 21$
- $-2x - 3x = 21 - 5$
- $-5x = 16$
- $x = -\frac{16}{5}$

## 3. Solving Fractional Equations

Find a common denominator to eliminate fractions.

**Example**: Solve $\frac{x}{2x + 1} = 4$
- Multiply both sides by $2x + 1$: $x = 4(2x + 1)$
- $x = 8x + 4$
- $x - 8x = 4$
- $-7x = 4$
- $x = -\frac{4}{7}$

**Example**: Solve $\frac{2}{x + 2} + \frac{3}{2x - 1} = 1$
- Common denominator: $(x + 2)(2x - 1)$
- $\frac{2(2x - 1) + 3(x + 2)}{(x + 2)(2x - 1)} = 1$
- $4x - 2 + 3x + 6 = (x + 2)(2x - 1)$
- $7x + 4 = 2x^2 + 3x - 2$
- $0 = 2x^2 - 4x - 6$
- Solve quadratic: $x = 3$ or $x = -1$

**Example**: Solve $\frac{x}{x + 2} = \frac{3}{x - 6}$
- Cross-multiply: $x(x - 6) = 3(x + 2)$
- $x^2 - 6x = 3x + 6$
- $x^2 - 9x - 6 = 0$
- Solve quadratic: $x = \frac{9 \pm \sqrt{105}}{2}$

## 4. Solving Simultaneous Linear Equations in Two Unknowns

Use substitution or elimination methods.

**Example**: Solve $2x + 3y = 7$, $x - y = 1$
- From second equation: $x = y + 1$
- Substitute: $2(y + 1) + 3y = 7$
- $2y + 2 + 3y = 7$
- $5y = 5$, $y = 1$
- $x = 1 + 1 = 2$
- Solution: $x = 2$, $y = 1$

## 5. Solving Simultaneous Equations (One Linear, One Non-Linear)

Substitute from linear into non-linear equation.

**Example**: Solve $x + y = 5$, $x^2 + y^2 = 13$
- From first equation: $y = 5 - x$
- Substitute: $x^2 + (5 - x)^2 = 13$
- $x^2 + 25 - 10x + x^2 = 13$
- $2x^2 - 10x + 12 = 0$
- $x^2 - 5x + 6 = 0$
- $(x - 2)(x - 3) = 0$
- $x = 2$ or $x = 3$
- Corresponding $y = 3$ or $y = 2$
- Solutions: $(2, 3)$ and $(3, 2)$

## 6. Solving Quadratic Equations

### Factorisation
**Example**: Solve $x^2 - 5x + 6 = 0$
- $(x - 2)(x - 3) = 0$
- $x = 2$ or $x = 3$

### Completing the Square
**Example**: Solve $x^2 + 6x + 2 = 0$
- $(x^2 + 6x + 9) + 2 - 9 = 0$
- $(x + 3)^2 - 7 = 0$
- $(x + 3)^2 = 7$
- $x + 3 = \pm \sqrt{7}$
- $x = -3 \pm \sqrt{7}$

### Quadratic Formula
For $ax^2 + bx + c = 0$:
\[ x = \frac{-b \pm \sqrt{b^2 - 4ac}}{2a} \]

**Example**: Solve $2x^2 - 4x - 6 = 0$
- $a = 2$, $b = -4$, $c = -6$
- $x = \frac{4 \pm \sqrt{16 + 48}}{4} = \frac{4 \pm \sqrt{64}}{4} = \frac{4 \pm 8}{4}$
- $x = 3$ or $x = -1$

## 7. Changing the Subject of Formulas

### Subject Appears Twice
**Example**: Make $x$ the subject of $y = \frac{x}{x + 1}$
- $y(x + 1) = x$
- $yx + y = x$
- $yx - x = -y$
- $x(y - 1) = -y$
- $x = \frac{-y}{y - 1} = \frac{y}{1 - y}$

### Subject with Power or Root
**Example**: Make $r$ the subject of $V = \frac{4}{3}\pi r^3$
- $r^3 = \frac{3V}{4\pi}$
- $r = \sqrt[3]{\frac{3V}{4\pi}}$

**Example**: Make $x$ the subject of $y = \sqrt{2x + 1}$
- $y^2 = 2x + 1$
- $2x = y^2 - 1$
- $x = \frac{y^2 - 1}{2}$

## Key Points to Remember
- Always check solutions in original equations
- State restrictions (values that make denominators zero)
- For quadratic formula, ensure correct identification of $a$, $b$, and $c$
- When changing subject, perform same operations on both sides
- For simultaneous equations, check all solutions satisfy both equations

These equation-solving skills are fundamental to algebra and higher mathematics.